* Task

Find all $f \colon \mathbb{R}^+ \to \mathbb{R}^+$ such that:
$P(x,y) \colon x(f(x) + f(y)) \geq (f(f(x)) + y)f(y) ~\forall~x,y \in \mathbb{R}^+$

* Exploration

** $Two(x) \colon x \geq f(f(x)) ~\forall~x \in \mathbb{R}^+$

$P(x,x) \colon 2x f(x) \geq (f(f(x)) + x) f(x)$
$2x \geq f(f(x)) + x$
$Two(x) \colon x \geq f(f(x)) ~\forall~x \in \mathbb{R}^+$

** $f(f(x)) = x~\forall~x \in \mathbb{R}^+$

$P(f(y),y) \colon f(f(y)) + f(y) \geq f(f(f(y))) + y$
Define sequence $\{a_n\}_{n=0}^\infty$
$a_0 = y$
$a_{n+1} = f(a_n)$
Then the following is true:
$a_{n+2} + a_{n+1} \geq a_{n+3} + a_n$
$a_{n+2} + a_{n+1} - a_n \geq a_{n+3}$
From $Two$ we know $a_n \geq a_{n+2}$

$a_{n+4} \leq a_{n+3} + a_{n+2} - a_{n+1} \leq 2a_{n+2} - a_n$
$a_{n+6} \leq 2a_{n+4} - a_{n+2} \leq 3a_{n+2} - 2a_n$

Want to prove: $a_{n+2k} \leq ka_{n+2} - (k-1)a_n$ via induction
$a_{n+2k+2} \leq ka_{n+4} - (k-1)a_{n+2} \leq 2ka_{n+2} - ka_n - (k-1)a_{n+2} = (k+1)a_{n+2} - ka_n$
Good

$0 < a_{2k} \leq kf(f(y)) - (k-1)y$
$(k-1)y < kf(f(y))$
$\dfrac{k-1}{k} < \dfrac{f(f(y))}{y}$
Therefore $1 \leq \dfrac{f(f(y))}{y}$
$y \leq f(f(y)) \stackrel{Two}{\leq} y$
Therefore $f(f(y)) = y~\forall~y \in \mathbb{R}^+$

** $f(x)=a/x~\forall~x \in \mathbb{R}+$

$P \colon x(f(x) + f(y)) \geq (x + y) f(y)$
$f(x) + f(y) \geq (x+y) \cdot \dfrac{f(y)}{x}$
$x + y = f(f(x)) + f(f(y)) \geq (f(x) + f(y)) \cdot \dfrac{f(f(y))}{f(x)} \geq (x + y) \cdot \dfrac{f(y)}{x} \dfrac{y}{f(x)}$
$xf(x) \geq yf(y)$
Therefore $f(x) = a/x~\forall~x \in \mathbb{R}^+$

$f(x) = a/x$ is a solution $\forall~a \in \mathbb{R}^+$


** Unsorted

$P(x,nx-f(f(x))) \colon x(f(x) + f(y)) \geq nx f(y)$
$f(x) + f(y) \geq n f(y)$
$f(x) \geq n f(nx - f(f(x)))$

$P(x,y) \colon x(f(x) + f(y)) \geq (f(f(x)) + y)f(y)$
$xf(x) + xf(y) \geq f(f(x))f(y) + yf(y)$
$f(y) \cdot (f(f(x)) - x + y) \leq xf(x)$
If  ----^-------- is positive:
$f(y) \leq \dfrac{xf(x)}{f(f(x)) - x + y}~\forall~y > x - f(f(x))$

$P\{f(x) = cf(x/c)\} \colon x(cf(x/c) + cf(y/c)) \stackrel{?}{\geq} (cf(f(x/c)) + y) cf(y/c)$
$x = cx, y = cy \colon cx(cf(x) + cf(y)) \stackrel{?}{\geq} (cf(f(x)) + cy)cf(y)$
$x(f(x) + f(y)) \stackrel{?}{\geq} (f(f(x)) + y)f(y)$
Therefore, if $f$ is a solution, so is $x \to cf(x/c)$
