* Task

Find all $f \colon \mathbb{N} \to \mathbb{N}$ such that
$f^{bf(a)}(a+1) = (a+1)f(b)~\forall~a,b \in \mathbb{N}$
Where $f^x$ represents composing $f$ with itself $x$ times

* Exploration

** No cycles

Suppose $a \geq 2 \colon f^n(a) = a$
Pretty obvious that $\text{Im}(f)$ is infinite
Note that every element of $a~\text{Im}(f)$ is reachable from $a$
Contradiction

Suppose $a=1$
If $n \geq 2$ do previous on $f(a)$

Remaining $f(1) = 1$
Plug in $a = b = 1$
$f(2) = 2$
Contradiction

** $f^x(a) = f^y(a) \implies x = y$

This is obvious from "No cycles"

** $f$ is injective

Suppose $f(b) = f(c)$
Then $f^{bf(a)}(a+1) = f^{cf(a)}(a+1)$
Then $bf(a) = cf(a)$
Then $b = c$
So we have injectivity!

** $1 \not \in \text{Im}(f)$

If it were, cycles would show up $f(b)=1$

** $\text{Im}(f) = \mathbb{N} \setminus \{1\}$, everything is reachable from $1$

$a+1 = f(x)$
$f^{bf(f(x)-1)}(f(x)) = f(x)f(b)$
$f^{bf(f(x)-1)+1}(x) = f^{xf(f(b)-1)+1}(b)$
$f^{f(f(x)-1)+1}(x) = f^{xf(f(1)-1)+1}(1)$
Since $1 \not \in \text{Im}(f)$ we know LHS exponent < RHS exponent when $x \neq 1$
Therefore every element from $\mathbb{N} \setminus \{1\}$ is reachable from $1$

** Unsorted

Let $I(n) = \text{distance from 1 to n}$
$f^{I(n)}(1) = n$

$a = f(a) - 1$
$f^{bf(f(a)-1)}(f(a)) = f(a)f(b)$
$bf(f(a)-1) + I(a) = af(f(b)-1) + I(b)$

$b=f^n(a)$
$f^n(a)f(f(a)-1) + I(a) = af(f^{n+1}(a)-1) + I(a) + n$
$f^n(a)f(f(a)-1) = af(f^{n+1}(a)-1) + n$
$n=1$
$f(a)f(f(a)-1) = af(f^2(a)-1)+1$
Therefore:
$M(a, f(a)) = 1$
$M(a, f(f(a)-1)) = 1$

$\lambda \mid a, n \implies \lambda \mid f^n(a)$
$\lambda \mid a \implies \left[ \lambda \mid n \iff \lambda \mid f^n(a) \right]$
This also works for negative $n$ as long as $a$ has the inverse

Let $f^n(1) = 2$
If $2 \mid n$ then $\lambda = 2, a = 2, n = -n$ implies $2 \mid 1$
So $2 \nmid n$
Suppose $n \geq 3$
Therefore $f^n(1) = 2 \mid f^{n-2}(1)$
Contradiction
Therefore $n = 1, f(1) = 2$

Induction
Suppose we showed $f(i) = i+1~\forall~i = 1, \dots, k$
We want to show $f(k+1) = k+2$
Let $f^x(1) = k+2$
$x \geq k+2 \implies f^x(1) \mid f^{x-k-2}(1)$ , contradiction
Therefore $x \leq k+1$
$f^k(1) = k+1$
So $x > k$
So $x = k+1$
So $f(k+1) = k+2$
Done!!

$a \mid b \implies a~\text{reaches}~b$


Suppose $f(x) = 2$
$xf(a) + yf(2a+1) = yf(a) + xf((a+1)f(y)-1)$


$f^{f(a)}(a+1) = (a+1)f(1)$
$f^{f(a) + f((a+1)f(1)-1)}(a+1) = (a+1)f(1)^2$
$f^{2f(a)}(a+1) = (a+1)f(2)$
$f^{2f(a) + f((a+1)f(2)-1)}(a+1) = (a+1)f(2)f(1)$
$f^{f(a) + 2f((a+1)f(1) - 1)}(a+1) = (a+1)f(1)f(2)$
Therefore:
$2f(a) + f((a+1)f(2)-1) = f(a) + 2f((a+1)f(1) - 1)$
$f(a) + f((a+1)f(2)-1) = 2f((a+1)f(1)-1)$

$f^{xf(a) + yf((a+1)f(x)-1)}(a+1) = f^{yf((a+1)f(x)-1)}((a+1)f(x)) = (a+1)f(x)f(y)$
Therefore:
$xf(a) + yf((a+1)f(x)-1) = yf(a) + xf((a+1)f(y)-1)$

$\forall~x, y~\exists~z \colon xf(a) + yf((a+1)f(x)-1) = zf(a)$
$z = f^{-1}(f(x) f(y))$
$x + yf((a+1)f(x)-1)/f(a) = z$
$f(x + yf((a+1)f(x)-1)/f(a)) = f(x)f(y)$

There might be some sense in saying $f(0)=1$
(comes from plugging in $b=0$)

$a+1 \stackrel{f^{f(a)}}{\to} (a+1) f(1) \stackrel{f^{f(a)}}{\to} (a+1) f(2) \dots$

Slight generalization:
$f^{cf(a)}((a+1)f(b)) = (a+1)f(b+c)$


# Suppose $f(a+1) = f(b+1)$
# Then $f^k(a+1) = f^k(b+1)~\forall~k \in \mathbb{N}$
# Let $k = kf(a)f(b)$
# $f^{kf(a)f(b)}(a+1) = f^{kf(a)f(b)}(b+1)$
# $(a+1)f(kf(b)) = (b+1)f(kf(a))$
# Generalization:
# $(a+1)^t f(kf(b)^t) = (b+1)^t f(kf(a)^t)$
# WLOG $a > b$



Suppose $f(a+1) = b+1$
$f^t(a+1) = f^{t-1}(b+1)$
Suppose $f(a) \mid t$ and $f(b) \mid t-1$
$(a+1)f(t/f(a)) = (b+1)f((t-1)/f(b))$


$f(a) = a+1$ is a solution


If $n \in \text{Im}(f)$ then $nk \in \text{Im}(f)~\forall~k \in \mathbb{N}$




** Case: $\exists~x \colon f(x)=1$

$a=x \colon f^b(x+1) = (x+1)f(b)$

$b=x \colon f^{xf(a)}(a+1) = a+1$
Therefore $f$ is surjective

TODO

